@prefix : <http://www.semanticweb.org/jamesegan/ontologies/2023/9/BasketballOntology/> .
@prefix cco: <http://www.ontologyrepository.com/CommonCoreOntologies/> .
@prefix owl: <http://www.w3.org/2002/07/owl#> .
@prefix obo: <http://purl.obolibrary.org/obo/> .
@prefix rdf: <http://www.w3.org/1999/02/22-rdf-syntax-ns#> .
@prefix xml: <http://www.w3.org/XML/1998/namespace> .
@prefix xsd: <http://www.w3.org/2001/XMLSchema#> .
@prefix rdfs: <http://www.w3.org/2000/01/rdf-schema#> .
@prefix skos: <http://www.w3.org/2004/02/skos/core#> .
@base <http://www.semanticweb.org/jamesegan/ontologies/2023/9/BasketballOntology/> .

<http://www.semanticweb.org/jamesegan/ontologies/2023/9/BasketballOntology> rdf:type owl:Ontology ;
                                                                             <http://purl.org/dc/elements/1.1/contributor> "James Egan" ;
                                                                             rdfs:label "BasketballOntology" .

#################################################################
#    Annotation properties
#################################################################

###  http://purl.obolibrary.org/obo/IAO_0000115
obo:IAO_0000115 rdf:type owl:AnnotationProperty ;
                rdfs:label "defintion"@en .


###  http://purl.org/dc/elements/1.1/contributor
dc:contributor rdf:type owl:AnnotationProperty .


###  http://purl.org/dc/elements/1.1/identifier
dc:identifier rdf:type owl:AnnotationProperty .


###  http://purl.org/dc/elements/1.1/license
dc:license rdf:type owl:AnnotationProperty .


###  http://www.w3.org/2004/02/skos/core#altLabel
skos:altLabel rdf:type owl:AnnotationProperty .


###  http://www.w3.org/2004/02/skos/core#definition
skos:definition rdf:type owl:AnnotationProperty .


###  http://www.w3.org/2004/02/skos/core#example
skos:example rdf:type owl:AnnotationProperty .


###  http://www.w3.org/2004/02/skos/core#prefLabel
skos:prefLabel rdf:type owl:AnnotationProperty .


###  http://www.w3.org/2004/02/skos/core#scopeNote
skos:scopeNote rdf:type owl:AnnotationProperty .

#################################################################
#    Object Properties
#################################################################




#################################################################
#    Classes
#################################################################


###  http://www.ontologyrepository.com/CommonCoreOntologies/Agent
cco:Agent rdf:type owl:Class ;
          cco:definition "A Material Entity that is capable of performing Planned Acts"@en ;
          cco:is_curated_in_ontology "http://www.ontologyrepository.com/CommonCoreOntologies/Mid/AgentOntology"^^xsd:anyURI ;
          rdfs:label "Agent"@en .


###  http://www.ontologyrepository.com/CommonCoreOntologies/Artifact
cco:Artifact rdf:type owl:Class ;
             cco:definition "A Material Entity that was designed by some Agent to realize a certain Function."@en ;
             cco:is_curated_in_ontology "http://www.ontologyrepository.com/CommonCoreOntologies/Mid/ArtifactOntology"^^xsd:anyURI ;
             rdfs:label "Material Artifact"@en .


###  http://www.ontologyrepository.com/CommonCoreOntologies/DescriptiveInformationContentEntity
cco:DescriptiveInformationContentEntity rdf:type owl:Class ;
                                        cco:definition "An Information Content Entity that consists of a set of propositions that describe some Entity."@en ;
                                        cco:is_curated_in_ontology "http://www.ontologyrepository.com/CommonCoreOntologies/Mid/InformationEntityOntology"^^xsd:anyURI ;
                                        rdfs:label "Descriptive Information Content Entity"@en .


###  http://www.ontologyrepository.com/CommonCoreOntologies/IntentionalAct
cco:IntentionalAct rdf:type owl:Class ;
                   cco:alternative_label "Intentional Act"@en ;
                   cco:definition "An Act in which at least one Agent plays a causative role and which is prescribed by some Directive Information Content Entity held by at least one of the Agents."@en ;
                   cco:is_curated_in_ontology "http://www.ontologyrepository.com/CommonCoreOntologies/Mid/EventOntology"^^xsd:anyURI ;
                   rdfs:label "Planned Act"@en .

###  http://www.ontologyrepository.com/CommonCoreOntologies/Facility
cco:Facility rdf:type owl:Class ;
             rdfs:subClassOf <http://www.ontologyrepository.com/CommonCoreOntologies/Artifact> ;
             cco:definition "A Material Artifact that is designed as a building or campus dedicated to some specific purpose."@en ;
             cco:is_curated_in_ontology "http://www.ontologyrepository.com/CommonCoreOntologies/Mid/ArtifactOntology"^^xsd:anyURI ;
             rdfs:label "Facility"@en .


###  http://www.ontologyrepository.com/CommonCoreOntologies/MeasurementInformationContentEntity
cco:MeasurementInformationContentEntity rdf:type owl:Class ;
                                        rdfs:subClassOf cco:DescriptiveInformationContentEntity ;
                                        cco:alternative_label "Measurement ICE"@en ;
                                        cco:definition "A Descriptive Information Content Entity that describes the extent, dimensions, quantity, or quality of an Entity relative to some standard."@en ;
                                        cco:is_curated_in_ontology "http://www.ontologyrepository.com/CommonCoreOntologies/Mid/InformationEntityOntology"^^xsd:anyURI ;
                                        rdfs:label "Measurement Information Content Entity"@en .


###  http://www.ontologyrepository.com/CommonCoreOntologies/MeasurementUnit
cco:MeasurementUnit rdf:type owl:Class ;
                    rdfs:subClassOf cco:DescriptiveInformationContentEntity ;
                    cco:definition "A Descriptive Information Content Entity that describes a definite magnitude of a physical quantity, defined and adopted by convention and/or by law, that is used as a standard for measurement of the same physical quantity."@en ;
                    cco:definition_source "https://en.wikipedia.org/w/index.php?title=Unit_of_measurement&oldid=1061038125"^^xsd:anyURI ;
                    cco:is_curated_in_ontology "http://www.ontologyrepository.com/CommonCoreOntologies/Mid/InformationEntityOntology"^^xsd:anyURI ;
                    rdfs:label "Measurement Unit"@en .


###  http://www.ontologyrepository.com/CommonCoreOntologies/OccupationRole
cco:OccupationRole rdf:type owl:Class ;
                   rdfs:subClassOf obo:BFO_0000023 ;
                   cco:definition "A Role that inheres in an Agent in virtue of the responsibilities that Agent is expected to fulfill within the context of some Act of Employment."@en ;
                   cco:is_curated_in_ontology "http://www.ontologyrepository.com/CommonCoreOntologies/Mid/AgentOntology"^^xsd:anyURI ;
                   rdfs:label "Occupation Role"@en .


###  http://purl.obolibrary.org/obo/BFO_0000035
obo:BFO_0000035 rdf:type owl:Class ;
                obo:BFO_0000179 "p-boundary" ;
                obo:BFO_0000180 "ProcessBoundary" ;
                obo:IAO_0000112 "the boundary between the 2nd and 3rd year of your life."@en ;
                obo:IAO_0000115 "p is a process boundary =Def. p is a temporal part of a process & p has no proper temporal parts. (axiom label in BFO2 Reference: [084-001])"@en ;
                obo:IAO_0000601 "Every process boundary occupies_temporal_region a zero-dimensional temporal region. (axiom label in BFO2 Reference: [085-002])"@en ;
                obo:IAO_0000602 "(forall (x) (if (ProcessBoundary x) (exists (y) (and (ZeroDimensionalTemporalRegion y) (occupiesTemporalRegion x y))))) // axiom label in BFO2 CLIF: [085-002] " ,
                                "(iff (ProcessBoundary a) (exists (p) (and (Process p) (temporalPartOf a p) (not (exists (b) (properTemporalPartOf b a)))))) // axiom label in BFO2 CLIF: [084-001] " ;
                rdfs:isDefinedBy obo:bfo.owl ;
                rdfs:label "process boundary"@en .


###  http://purl.obolibrary.org/obo/BFO_0000023
obo:BFO_0000023 rdf:type owl:Class ;
                rdfs:subClassOf obo:BFO_0000017 ;
                obo:BFO_0000179 "role" ;
                obo:BFO_0000180 "Role" ;
                obo:IAO_0000112 "John’s role of husband to Mary is dependent on Mary’s role of wife to John, and both are dependent on the object aggregate comprising John and Mary as member parts joined together through the relational quality of being married."@en ,
                                "the priest role"@en ,
                                "the role of a boundary to demarcate two neighboring administrative territories"@en ,
                                "the role of a building in serving as a military target"@en ,
                                "the role of a stone in marking a property boundary"@en ,
                                "the role of subject in a clinical trial"@en ,
                                "the student role"@en ;
                obo:IAO_0000116 "BFO 2 Reference: One major family of examples of non-rigid universals involves roles, and ontologies developed for corresponding administrative purposes may consist entirely of representatives of entities of this sort. Thus ‘professor’, defined as follows,b instance_of professor at t =Def. there is some c, c instance_of professor role & c inheres_in b at t.denotes a non-rigid universal and so also do ‘nurse’, ‘student’, ‘colonel’, ‘taxpayer’, and so forth. (These terms are all, in the jargon of philosophy, phase sortals.) By using role terms in definitions, we can create a BFO conformant treatment of such entities drawing on the fact that, while an instance of professor may be simultaneously an instance of trade union member, no instance of the type professor role is also (at any time) an instance of the type trade union member role (any more than any instance of the type color is at any time an instance of the type length).If an ontology of employment positions should be defined in terms of roles following the above pattern, this enables the ontology to do justice to the fact that individuals instantiate the corresponding universals –  professor, sergeant, nurse – only during certain phases in their lives."@en ;
                obo:IAO_0000600 "b is a role means: b is a realizable entity & b exists because there is some single bearer that is in some special physical, social, or institutional set of circumstances in which this bearer does not have to be& b is not such that, if it ceases to exist, then the physical make-up of the bearer is thereby changed. (axiom label in BFO2 Reference: [061-001])"@en ;
                obo:IAO_0000602 "(forall (x) (if (Role x) (RealizableEntity x))) // axiom label in BFO2 CLIF: [061-001] " ;
                rdfs:isDefinedBy obo:bfo.owl ;
                rdfs:label "role"@en .


###  http://purl.obolibrary.org/obo/BFO_0000019
obo:BFO_0000019 rdf:type owl:Class ;
                obo:BFO_0000179 "quality" ;
                obo:BFO_0000180 "Quality" ;
                obo:IAO_0000112 "the ambient temperature of this portion of air"@en ,
                                "the color of a tomato"@en ,
                                "the length of the circumference of your waist"@en ,
                                "the mass of this piece of gold."@en ,
                                "the shape of your nose"@en ,
                                "the shape of your nostril"@en ;
                obo:IAO_0000600 "a quality is a specifically dependent continuant that, in contrast to roles and dispositions, does not require any further process in order to be realized. (axiom label in BFO2 Reference: [055-001])"@en ;
                obo:IAO_0000601 "If an entity is a quality at any time that it exists, then it is a quality at every time that it exists. (axiom label in BFO2 Reference: [105-001])"@en ;
                obo:IAO_0000602 "(forall (x) (if (Quality x) (SpecificallyDependentContinuant x))) // axiom label in BFO2 CLIF: [055-001] " ,
                                "(forall (x) (if (exists (t) (and (existsAt x t) (Quality x))) (forall (t_1) (if (existsAt x t_1) (Quality x))))) // axiom label in BFO2 CLIF: [105-001] " ;
                rdfs:isDefinedBy obo:bfo.owl ;
                rdfs:label "quality"@en .


###  http://www.semanticweb.org/jamesegan/ontologies/2023/9/BasketballOntology/BBO_000001
<http://www.semanticweb.org/jamesegan/ontologies/2023/9/BasketballOntology/BBO_000001> rdf:type owl:Class ;
                                                                                       rdfs:subClassOf <http://www.ontologyrepository.com/CommonCoreOntologies/IntentionalAct> ;
                                                                                       obo:IAO_0000115 "an Intentional Act that is performed by a person during a match."@en ;
                                                                                       rdfs:comment "These actions can range from playing actions (like shooting, passing, or dribbling) performed by players, to strategic decisions and instructions given by coaches, to rulings and decisions made by referees."@en ;
                                                                                       rdfs:label "intentionalMatchAct"@en .


###  http://www.semanticweb.org/jamesegan/ontologies/2023/9/BasketballOntology/BBO_000002
<http://www.semanticweb.org/jamesegan/ontologies/2023/9/BasketballOntology/BBO_000002> rdf:type owl:Class ;
                                                                                       rdfs:subClassOf <http://www.semanticweb.org/jamesegan/ontologies/2023/9/BasketballOntology/BBO_000001> ;
                                                                                       obo:IAO_0000115 "an intentionalMatchAct that represents any action performed intentionally by a player during a match."@en ;
                                                                                       rdfs:label "playerAct"@en .

###  http://www.semanticweb.org/jamesegan/ontologies/2023/9/BasketballOntology/BBO_000003
<http://www.semanticweb.org/jamesegan/ontologies/2023/9/BasketballOntology/BBO_000003> rdf:type owl:Class ;
                                                                                       rdfs:subClassOf <http://www.semanticweb.org/jamesegan/ontologies/2023/9/BasketballOntology/BBO_000002> ;
                                                                                       obo:IAO_0000115 "a playerAct that involves actions performed by players actively participating in the match."@en ;
                                                                                       rdfs:label "selectedPlayerAct"@en .


###  http://www.semanticweb.org/jamesegan/ontologies/2023/9/BasketballOntology/BBO_000004
:BBO_000004 rdf:type owl:Class ;
            rdfs:subClassOf <http://www.semanticweb.org/jamesegan/ontologies/2023/9/BasketballOntology/BBO_000003> ;
            obo:IAO_0000115 "a selectedPlayerAct that involves actions executed by players of the team that currently has control of the ball."@en ;
            rdfs:label "inPossessionAct"@en .


###  http://www.semanticweb.org/jamesegan/ontologies/2023/9/BasketballOntology/BBO_000005
:BBO_000005 rdf:type owl:Class ;
            rdfs:subClassOf <http://www.semanticweb.org/jamesegan/ontologies/2023/9/BasketballOntology/BBO_000004> ;
            obo:IAO_0000115 "an inPossessionAct that involves a player maintaining control of the ball during the match."@en ;
            rdfs:label "onBallAct"@en .


###  http://www.semanticweb.org/jamesegan/ontologies/2023/9/BasketballOntology/BBO_000006
:BBO_000006 rdf:type owl:Class ;
            rdfs:subClassOf <http://www.semanticweb.org/jamesegan/ontologies/2023/9/BasketballOntology/BBO_000005> ;
            obo:IAO_0000115 "an onBallAct that is performed by a player when they attempt to propel the ball into the hoop."@en ;
            rdfs:label "shotAct"@en .

###  http://www.semanticweb.org/jamesegan/ontologies/2023/9/BasketballOntology/BBO_000008
:BBO_000008 rdf:type owl:Class ;
            rdfs:subClassOf <http://www.semanticweb.org/jamesegan/ontologies/2023/9/BasketballOntology/BBO_000006> ;
            obo:IAO_0000115 "a shotAct by a player located behind the free throw line that is unnaposed by the other team and is awarded as a penalty ."@en ;
            rdfs:label "freeThrowShotAct"@en .


###  http://www.semanticweb.org/jamesegan/ontologies/2023/9/BasketballOntology/BBO_000009
:BBO_000009 rdf:type owl:Class ;
            rdfs:subClassOf <http://www.semanticweb.org/jamesegan/ontologies/2023/9/BasketballOntology/BBO_000006> ;
            obo:IAO_0000115 "a fieldGoalShotAct by a player located behind the three point line."@en ;
            rdfs:label "threePointShotAct"@en .


###  http://www.semanticweb.org/jamesegan/ontologies/2023/9/BasketballOntology/BBO_000010
:BBO_000010 rdf:type owl:Class ;
            rdfs:subClassOf <http://www.ontologyrepository.com/CommonCoreOntologies/OccupationRole> ;
            obo:IAO_0000115 "an Occupation Role that inheres in a person who is a professional player for a basketball team."@en ;
            rdfs:label "basketballPlayerRole"@en .


###  http://www.semanticweb.org/jamesegan/ontologies/2023/9/BasketballOntology/BBO_000011
:BBO_000011 rdf:type owl:Class ;
            rdfs:subClassOf <http://www.semanticweb.org/jamesegan/ontologies/2023/9/BasketballOntology/BBO_000010> ;
            obo:IAO_0000115 "a basketballPlayerRole that inheres in a person who is a player for the NBA."@en ;
            rdfs:label "NBATeamPlayerRole"@en .


###  http://www.semanticweb.org/jamesegan/ontologies/2023/9/BasketballOntology/BBO_000012
:BBO_000012 rdf:type owl:Class ;
            rdfs:subClassOf <http://www.semanticweb.org/jamesegan/ontologies/2023/9/BasketballOntology/BBO_000005> ;
            obo:IAO_0000115 "an onBallAct that is performed by a player when they tap the ball on the floor."@en ;
            rdfs:label "dribbleAct"@en .


###  http://www.semanticweb.org/jamesegan/ontologies/2023/9/BasketballOntology/BBO_000013
:BBO_000013 rdf:type owl:Class ;
            rdfs:subClassOf <http://www.semanticweb.org/jamesegan/ontologies/2023/9/BasketballOntology/BBO_000005> ;
            obo:IAO_0000115 "an onBallAct that is performed by a player when they throw or hand the ball to another player on the same team."@en ;
            rdfs:label "passAct"@en .


##  http://www.semanticweb.org/jamesegan/ontologies/2023/9/BasketballOntology/BBO_000014
:BBO_000014 rdf:type owl:Class ;
            rdfs:subClassOf <http://www.semanticweb.org/jamesegan/ontologies/2023/9/BasketballOntology/BBO_000004> ;
            obo:IAO_0000115 "an inPossessionAct that involves players not controlling the ball during the match."@en ;
            rdfs:label "offBallAct"@en .


###  http://www.semanticweb.org/jamesegan/ontologies/2023/9/BasketballOntology/BBO_000015
:BBO_000015 rdf:type owl:Class ;
            rdfs:subClassOf <http://www.semanticweb.org/jamesegan/ontologies/2023/9/BasketballOntology/BBO_000003> ;
            obo:IAO_0000115 "a selectedPlayerAct that involves actions executed by players of the team that currently does not have control of the ball."@en ;
            rdfs:label "outOfPossessionAct"@en .


###  http://www.semanticweb.org/jamesegan/ontologies/2023/9/BasketballOntology/BBO_000016
<http://www.semanticweb.org/jamesegan/ontologies/2023/9/BasketballOntology/BBO_000016> rdf:type owl:Class ;
            rdfs:subClassOf obo:BFO_0000035 ;
            obo:IAO_0000115 "A process boundary that marks the beginning of a basketball game event."@en ;
            rdfs:label "GameStart"@en .

###  http://www.semanticweb.org/jamesegan/ontologies/2023/9/BasketballOntology/BBO_000017
:BBO_000017 rdf:type owl:Class ;
            rdfs:subClassOf obo:BFO_0000035 ;
            obo:IAO_0000115 "A process boundary that marks the end of a basketball game event."@en ;
            rdfs:label "GameEnd"@en .


###  http://www.semanticweb.org/jamesegan/ontologies/2023/9/BasketballOntology/BBO_000018
:BBO_000018 rdf:type owl:Class ;
            rdfs:subClassOf obo:BFO_0000035 ;
            obo:IAO_0000115 "A process boundary that marks the beginning of the first quarter of a basketball game event."@en ;
            rdfs:label "QuarterOneStart"@en .


###  http://www.semanticweb.org/jamesegan/ontologies/2023/9/BasketballOntology/BBO_000019
:BBO_000019 rdf:type owl:Class ;
            rdfs:subClassOf obo:BFO_0000035 ;
            obo:IAO_0000115 "A process boundary that marks the end of the first quarter of a basketball game event."@en ;
            rdfs:label "QuarterOneEnd"@en .


###  http://www.semanticweb.org/jamesegan/ontologies/2023/9/BasketballOntology/BBO_000020
:BBO_000020 rdf:type owl:Class ;
            rdfs:subClassOf obo:BFO_0000035 ;
            obo:IAO_0000115 "A process boundary that marks the beginning of the second quarter of a basketball game event."@en ;
            rdfs:label "QuarterTwoStart"@en .


###  http://www.semanticweb.org/jamesegan/ontologies/2023/9/BasketballOntology/BBO_000021
:BBO_000021 rdf:type owl:Class ;
            rdfs:subClassOf obo:BFO_0000035 ;
            obo:IAO_0000115 "A process boundary that marks the end of the second quarter of a basketball game event."@en ;
            rdfs:label "QuarterTwoEnd"@en .


###  http://www.semanticweb.org/jamesegan/ontologies/2023/9/BasketballOntology/BBO_000022
:BBO_000022 rdf:type owl:Class ;
            rdfs:subClassOf obo:BFO_0000035 ;
            obo:IAO_0000115 "A process boundary that marks the beginning of the third quarter of a basketball game event."@en ;
            rdfs:label "QuarterThreeStart"@en .


###  http://www.semanticweb.org/jamesegan/ontologies/2023/9/BasketballOntology/BBO_000023
:BBO_000023 rdf:type owl:Class ;
            rdfs:subClassOf obo:BFO_0000035 ;
            obo:IAO_0000115 "A process boundary that marks the end of the third quarter of a basketball game event."@en ;
            rdfs:label "QuarterThreeEnd"@en .


###  http://www.semanticweb.org/jamesegan/ontologies/2023/9/BasketballOntology/BBO_000024
:BBO_000024 rdf:type owl:Class ;
            rdfs:subClassOf obo:BFO_0000035 ;
            obo:IAO_0000115 "A process boundary that marks the beginning of the fourth quarter of a basketball game event."@en ;
            rdfs:label "QuarterFourStart"@en .


###  http://www.semanticweb.org/jamesegan/ontologies/2023/9/BasketballOntology/BBO_000025
:BBO_000025 rdf:type owl:Class ;
            rdfs:subClassOf obo:BFO_0000035 ;
            obo:IAO_0000115 "A process boundary that marks the end of the fourth quarter of a basketball game event."@en ;
            rdfs:label "QuarterFourEnd"@en .


###  http://www.semanticweb.org/jamesegan/ontologies/2023/9/BasketballOntology/BBO_000026
:BBO_000026 rdf:type owl:Class ;
            rdfs:subClassOf obo:BFO_0000019 ;
            obo:IAO_0000115 "A quality that a player has measured by units like inches."@en ;
            rdfs:label "Height"@en .


###  http://www.semanticweb.org/jamesegan/ontologies/2023/9/BasketballOntology/BBO_000027
:BBO_000027 rdf:type owl:Class ;
            rdfs:subClassOf obo:BFO_0000019 ;
            obo:IAO_0000115 "A quality that a player has measured by units like pounds."@en ;
            rdfs:label "Weight"@en .


###  http://www.semanticweb.org/jamesegan/ontologies/2023/9/BasketballOntology/BBO_000028
:BBO_000028 rdf:type owl:Class ;
            rdfs:subClassOf cco:Artifact ;
            obo:IAO_0000115 "A material artifact used by selected players to perform on ball acts."@en ;
            rdfs:label "Basketball"@en .


###  http://www.semanticweb.org/jamesegan/ontologies/2023/9/BasketballOntology/BBO_000029
:BBO_000029 rdf:type owl:Class ;
            rdfs:subClassOf cco:Facility ;
            obo:IAO_0000115 "A facility with a basketball court that is designated to host basketball matches with an audience"@en ;
            rdfs:label "BasketballStadium"@en .


###  http://www.semanticweb.org/jamesegan/ontologies/2023/9/BasketballOntology/BBO_000030
:BBO_000030 rdf:type owl:Class ;
                rdfs:subClassOf obo:BFO_0000023 ;
                obo:IAO_0000115 "a role that inheres in a player with a specific position in a basketball game"@en ;
                rdfs:label "BasketballPlayerRole"@en .


###  http://www.semanticweb.org/jamesegan/ontologies/2023/9/BasketballOntology/BBO_000031
:BBO_000030 rdf:type owl:Class ;
                rdfs:subClassOf <http://www.semanticweb.org/jamesegan/ontologies/2023/9/BasketballOntology/BBO_000030> ;
                obo:IAO_0000115 "a role that inheres in a player who leads the team's offence"@en ;
                rdfs:label "PointGuardRole"@en .


###  http://www.semanticweb.org/jamesegan/ontologies/2023/9/BasketballOntology/BBO_000031
:BBO_000031 rdf:type owl:Class ;
                rdfs:subClassOf <http://www.semanticweb.org/jamesegan/ontologies/2023/9/BasketballOntology/BBO_000030> ;
                obo:IAO_0000115 "a role that inheres in a player who"@en ;
                rdfs:label "ShootingGuardRole"@en .


###  http://www.semanticweb.org/jamesegan/ontologies/2023/9/BasketballOntology/BBO_000032
:BBO_000032 rdf:type owl:Class ;
                rdfs:subClassOf <http://www.semanticweb.org/jamesegan/ontologies/2023/9/BasketballOntology/BBO_000030> ;
                obo:IAO_0000115 "a role that inheres in a player who"@en ;
                rdfs:label "SmallForwardRole"@en .


###  http://www.semanticweb.org/jamesegan/ontologies/2023/9/BasketballOntology/BBO_000033
:BBO_000033 rdf:type owl:Class ;
                rdfs:subClassOf <http://www.semanticweb.org/jamesegan/ontologies/2023/9/BasketballOntology/BBO_000030> ;
                obo:IAO_0000115 "a role that inheres in a player who"@en ;
                rdfs:label "PowerForwardRole"@en .


###  http://www.semanticweb.org/jamesegan/ontologies/2023/9/BasketballOntology/BBO_000034
:BBO_000034 rdf:type owl:Class ;
                rdfs:subClassOf <http://www.semanticweb.org/jamesegan/ontologies/2023/9/BasketballOntology/BBO_000030> ;
                obo:IAO_0000115 "a role that inheres in a player who"@en ;
                rdfs:label "CenterRole"@en .
###  Generated by the OWL API (version 4.5.25.2023-02-15T19:15:49Z) https://github.com/owlcs/owlapi
