@prefix : <http://www.semanticweb.org/jamesegan/ontologies/2023/9/BasketballOntology/> .
@prefix cco: <http://www.ontologyrepository.com/CommonCoreOntologies/> .
@prefix owl: <http://www.w3.org/2002/07/owl#> .
@prefix obo: <http://purl.obolibrary.org/obo/> .
@prefix rdf: <http://www.w3.org/1999/02/22-rdf-syntax-ns#> .
@prefix xml: <http://www.w3.org/XML/1998/namespace> .
@prefix xsd: <http://www.w3.org/2001/XMLSchema#> .
@prefix rdfs: <http://www.w3.org/2000/01/rdf-schema#> .
@prefix skos: <http://www.w3.org/2004/02/skos/core#> .
@base <http://www.semanticweb.org/jamesegan/ontologies/2023/9/BasketballOntology/> .

<http://www.semanticweb.org/jamesegan/ontologies/2023/9/BasketballOntology> rdf:type owl:Ontology ;
                                                                             <http://purl.org/dc/elements/1.1/contributor> "James Egan" ;
                                                                             rdfs:label "BasketballOntology" .

#################################################################
#    Annotation properties
#################################################################

###  http://purl.obolibrary.org/obo/IAO_0000115
obo:IAO_0000115 rdf:type owl:AnnotationProperty ;
                rdfs:label "defintion"@en .


###  http://purl.org/dc/elements/1.1/contributor
dc:contributor rdf:type owl:AnnotationProperty .


###  http://purl.org/dc/elements/1.1/identifier
dc:identifier rdf:type owl:AnnotationProperty .


###  http://purl.org/dc/elements/1.1/license
dc:license rdf:type owl:AnnotationProperty .


###  http://www.w3.org/2004/02/skos/core#altLabel
skos:altLabel rdf:type owl:AnnotationProperty .


###  http://www.w3.org/2004/02/skos/core#definition
skos:definition rdf:type owl:AnnotationProperty .


###  http://www.w3.org/2004/02/skos/core#example
skos:example rdf:type owl:AnnotationProperty .


###  http://www.w3.org/2004/02/skos/core#prefLabel
skos:prefLabel rdf:type owl:AnnotationProperty .


###  http://www.w3.org/2004/02/skos/core#scopeNote
skos:scopeNote rdf:type owl:AnnotationProperty .

#################################################################
#    Object Properties
#################################################################




#################################################################
#    Classes
#################################################################


###  http://www.ontologyrepository.com/CommonCoreOntologies/Agent
cco:Agent rdf:type owl:Class ;
          cco:definition "A Material Entity that is capable of performing Planned Acts"@en ;
          cco:is_curated_in_ontology "http://www.ontologyrepository.com/CommonCoreOntologies/Mid/AgentOntology"^^xsd:anyURI ;
          rdfs:label "Agent"@en .


###  http://www.ontologyrepository.com/CommonCoreOntologies/Artifact
cco:Artifact rdf:type owl:Class ;
             cco:definition "A Material Entity that was designed by some Agent to realize a certain Function."@en ;
             cco:is_curated_in_ontology "http://www.ontologyrepository.com/CommonCoreOntologies/Mid/ArtifactOntology"^^xsd:anyURI ;
             rdfs:label "Material Artifact"@en .


###  http://www.ontologyrepository.com/CommonCoreOntologies/DescriptiveInformationContentEntity
cco:DescriptiveInformationContentEntity rdf:type owl:Class ;
                                        cco:definition "An Information Content Entity that consists of a set of propositions that describe some Entity."@en ;
                                        cco:is_curated_in_ontology "http://www.ontologyrepository.com/CommonCoreOntologies/Mid/InformationEntityOntology"^^xsd:anyURI ;
                                        rdfs:label "Descriptive Information Content Entity"@en .


###  http://www.ontologyrepository.com/CommonCoreOntologies/IntentionalAct
cco:IntentionalAct rdf:type owl:Class ;
                   cco:alternative_label "Intentional Act"@en ;
                   cco:definition "An Act in which at least one Agent plays a causative role and which is prescribed by some Directive Information Content Entity held by at least one of the Agents."@en ;
                   cco:is_curated_in_ontology "http://www.ontologyrepository.com/CommonCoreOntologies/Mid/EventOntology"^^xsd:anyURI ;
                   rdfs:label "Planned Act"@en .

###  http://www.ontologyrepository.com/CommonCoreOntologies/Facility
cco:Facility rdf:type owl:Class ;
             rdfs:subClassOf <http://www.ontologyrepository.com/CommonCoreOntologies/Artifact> ;
             cco:definition "A Material Artifact that is designed as a building or campus dedicated to some specific purpose."@en ;
             cco:is_curated_in_ontology "http://www.ontologyrepository.com/CommonCoreOntologies/Mid/ArtifactOntology"^^xsd:anyURI ;
             rdfs:label "Facility"@en .


###  http://www.ontologyrepository.com/CommonCoreOntologies/MeasurementInformationContentEntity
cco:MeasurementInformationContentEntity rdf:type owl:Class ;
                                        owl:equivalentClass [ owl:intersectionOf ( cco:DescriptiveInformationContentEntity
                                                                                   [ rdf:type owl:Restriction ;
                                                                                     owl:onProperty cco:is_a_measurement_of ;
                                                                                     owl:someValuesFrom obo:BFO_0000001
                                                                                   ]
                                                                                 ) ;
                                                              rdf:type owl:Class
                                                            ] ;
                                        owl:disjointWith cco:RepresentationalInformationContentEntity ;
                                        cco:alternative_label "Measurement ICE"@en ;
                                        cco:definition "A Descriptive Information Content Entity that describes the extent, dimensions, quantity, or quality of an Entity relative to some standard."@en ;
                                        cco:is_curated_in_ontology "http://www.ontologyrepository.com/CommonCoreOntologies/Mid/InformationEntityOntology"^^xsd:anyURI ;
                                        rdfs:label "Measurement Information Content Entity"@en .



###  http://www.ontologyrepository.com/CommonCoreOntologies/OccupationRole
cco:OccupationRole rdf:type owl:Class ;
                   cco:definition "A Role that inheres in an Agent in virtue of the responsibilities that Agent is expected to fulfill within the context of some Act of Employment."@en ;
                   cco:is_curated_in_ontology "http://www.ontologyrepository.com/CommonCoreOntologies/Mid/AgentOntology"^^xsd:anyURI ;
                   rdfs:label "Occupation Role"@en .


###  http://purl.obolibrary.org/obo/BFO_0000035
obo:BFO_0000035 rdf:type owl:Class ;
                obo:BFO_0000179 "p-boundary" ;
                obo:BFO_0000180 "ProcessBoundary" ;
                obo:IAO_0000112 "the boundary between the 2nd and 3rd year of your life."@en ;
                obo:IAO_0000115 "p is a process boundary =Def. p is a temporal part of a process & p has no proper temporal parts. (axiom label in BFO2 Reference: [084-001])"@en ;
                obo:IAO_0000601 "Every process boundary occupies_temporal_region a zero-dimensional temporal region. (axiom label in BFO2 Reference: [085-002])"@en ;
                obo:IAO_0000602 "(forall (x) (if (ProcessBoundary x) (exists (y) (and (ZeroDimensionalTemporalRegion y) (occupiesTemporalRegion x y))))) // axiom label in BFO2 CLIF: [085-002] " ,
                                "(iff (ProcessBoundary a) (exists (p) (and (Process p) (temporalPartOf a p) (not (exists (b) (properTemporalPartOf b a)))))) // axiom label in BFO2 CLIF: [084-001] " ;
                rdfs:isDefinedBy obo:bfo.owl ;
                rdfs:label "process boundary"@en .


###  http://purl.obolibrary.org/obo/BFO_0000019
obo:BFO_0000019 rdf:type owl:Class ;
                obo:BFO_0000179 "quality" ;
                obo:BFO_0000180 "Quality" ;
                obo:IAO_0000112 "the ambient temperature of this portion of air"@en ,
                                "the color of a tomato"@en ,
                                "the length of the circumference of your waist"@en ,
                                "the mass of this piece of gold."@en ,
                                "the shape of your nose"@en ,
                                "the shape of your nostril"@en ;
                obo:IAO_0000600 "a quality is a specifically dependent continuant that, in contrast to roles and dispositions, does not require any further process in order to be realized. (axiom label in BFO2 Reference: [055-001])"@en ;
                obo:IAO_0000601 "If an entity is a quality at any time that it exists, then it is a quality at every time that it exists. (axiom label in BFO2 Reference: [105-001])"@en ;
                obo:IAO_0000602 "(forall (x) (if (Quality x) (SpecificallyDependentContinuant x))) // axiom label in BFO2 CLIF: [055-001] " ,
                                "(forall (x) (if (exists (t) (and (existsAt x t) (Quality x))) (forall (t_1) (if (existsAt x t_1) (Quality x))))) // axiom label in BFO2 CLIF: [105-001] " ;
                rdfs:isDefinedBy obo:bfo.owl ;
                rdfs:label "quality"@en .


###  http://www.semanticweb.org/jamesegan/ontologies/2023/9/BasketballOntology/BBO_000001
<http://www.semanticweb.org/jamesegan/ontologies/2023/9/BasketballOntology/BBO_000001> rdf:type owl:Class ;
                                                                                       rdfs:subClassOf <http://www.ontologyrepository.com/CommonCoreOntologies/IntentionalAct> ;
                                                                                       obo:IAO_0000115 "an Intentional Act that is performed by a person during a match."@en ;
                                                                                       rdfs:comment "These actions can range from playing actions (like shooting, passing, or dribbling) performed by players, to strategic decisions and instructions given by coaches, to rulings and decisions made by referees."@en ;
                                                                                       rdfs:label "intentionalMatchAct"@en .


###  http://www.semanticweb.org/jamesegan/ontologies/2023/9/BasketballOntology/BBO_000002
<http://www.semanticweb.org/jamesegan/ontologies/2023/9/BasketballOntology/BBO_000002> rdf:type owl:Class ;
                                                                                       rdfs:subClassOf <http://www.semanticweb.org/jamesegan/ontologies/2023/9/BasketballOntology/BBO_000001> ;
                                                                                       obo:IAO_0000115 "an intentionalMatchAct that represents any action performed intentionally by a player during a match."@en ;
                                                                                       rdfs:label "playerAct"@en .

###  http://www.semanticweb.org/jamesegan/ontologies/2023/9/BasketballOntology/BBO_000003
<http://www.semanticweb.org/jamesegan/ontologies/2023/9/BasketballOntology/BBO_000003> rdf:type owl:Class ;
                                                                                       rdfs:subClassOf <http://www.semanticweb.org/jamesegan/ontologies/2023/9/BasketballOntology/BBO_000002> ;
                                                                                       obo:IAO_0000115 "a playerAct that involves actions performed by players actively participating in the match."@en ;
                                                                                       rdfs:label "selectedPlayerAct"@en .


###  http://www.semanticweb.org/jamesegan/ontologies/2023/9/BasketballOntology/BBO_000004
:BBO_000004 rdf:type owl:Class ;
            rdfs:subClassOf <http://www.semanticweb.org/jamesegan/ontologies/2023/9/BasketballOntology/BBO_000003> ;
            obo:IAO_0000115 "a selectedPlayerAct that involves actions executed by players of the team that currently has control of the ball."@en ;
            rdfs:label "inPossessionAct"@en .


###  http://www.semanticweb.org/jamesegan/ontologies/2023/9/BasketballOntology/BBO_000005
:BBO_000005 rdf:type owl:Class ;
            rdfs:subClassOf <http://www.semanticweb.org/jamesegan/ontologies/2023/9/BasketballOntology/BBO_000004> ;
            obo:IAO_0000115 "an inPossessionAct that involves a player maintaining control of the ball during the match."@en ;
            rdfs:label "onBallAct"@en .


###  http://www.semanticweb.org/jamesegan/ontologies/2023/9/BasketballOntology/BBO_000006
:BBO_000006 rdf:type owl:Class ;
            rdfs:subClassOf <http://www.semanticweb.org/jamesegan/ontologies/2023/9/BasketballOntology/BBO_000005> ;
            obo:IAO_0000115 "an onBallAct that is performed by a player when they attempt to propel the ball into the hoop."@en ;
            rdfs:label "shotAct"@en .

###  http://www.semanticweb.org/jamesegan/ontologies/2023/9/BasketballOntology/BBO_000008
:BBO_000008 rdf:type owl:Class ;
            rdfs:subClassOf <http://www.semanticweb.org/jamesegan/ontologies/2023/9/BasketballOntology/BBO_000006> ;
            obo:IAO_0000115 "a shotAct by a player located behind the free throw line that is unnaposed by the other team and is awarded as a penalty ."@en ;
            rdfs:label "freeThrowShotAct"@en .


###  http://www.semanticweb.org/jamesegan/ontologies/2023/9/BasketballOntology/BBO_000009
:BBO_000009 rdf:type owl:Class ;
            rdfs:subClassOf <http://www.semanticweb.org/jamesegan/ontologies/2023/9/BasketballOntology/BBO_000006> ;
            obo:IAO_0000115 "a fieldGoalShotAct by a player located behind the three point line."@en ;
            rdfs:label "threePointShotAct"@en .


###  http://www.semanticweb.org/jamesegan/ontologies/2023/9/BasketballOntology/BBO_000010
:BBO_000010 rdf:type owl:Class ;
            rdfs:subClassOf <http://www.ontologyrepository.com/CommonCoreOntologies/OccupationRole> ;
            obo:IAO_0000115 "an Occupation Role that inheres in a person who is a professional player for a basketball team."@en ;
            rdfs:label "basketballPlayerRole"@en .


###  http://www.semanticweb.org/jamesegan/ontologies/2023/9/BasketballOntology/BBO_000011
:BBO_000011 rdf:type owl:Class ;
            rdfs:subClassOf <http://www.semanticweb.org/jamesegan/ontologies/2023/9/BasketballOntology/BBO_000010> ;
            obo:IAO_0000115 "a basketballPlayerRole that inheres in a person who is a player for the NBA."@en ;
            rdfs:label "NBATeamPlayerRole"@en .


###  http://www.semanticweb.org/jamesegan/ontologies/2023/9/BasketballOntology/BBO_000012
:BBO_000012 rdf:type owl:Class ;
            rdfs:subClassOf <http://www.semanticweb.org/jamesegan/ontologies/2023/9/BasketballOntology/BBO_000005> ;
            obo:IAO_0000115 "an onBallAct that is performed by a player when they tap the ball on the floor."@en ;
            rdfs:label "dribbleAct"@en .


###  http://www.semanticweb.org/jamesegan/ontologies/2023/9/BasketballOntology/BBO_000013
:BBO_000013 rdf:type owl:Class ;
            rdfs:subClassOf <http://www.semanticweb.org/jamesegan/ontologies/2023/9/BasketballOntology/BBO_000005> ;
            obo:IAO_0000115 "an onBallAct that is performed by a player when they throw or hand the ball to another player on the same team."@en ;
            rdfs:label "passAct"@en .


##  http://www.semanticweb.org/jamesegan/ontologies/2023/9/BasketballOntology/BBO_000014
:BBO_000014 rdf:type owl:Class ;
            rdfs:subClassOf <http://www.semanticweb.org/jamesegan/ontologies/2023/9/BasketballOntology/BBO_000004> ;
            obo:IAO_0000115 "an inPossessionAct that involves players not controlling the ball during the match."@en ;
            rdfs:label "offBallAct"@en .


###  http://www.semanticweb.org/jamesegan/ontologies/2023/9/BasketballOntology/BBO_000015
:BBO_000015 rdf:type owl:Class ;
            rdfs:subClassOf <http://www.semanticweb.org/jamesegan/ontologies/2023/9/BasketballOntology/BBO_000003> ;
            obo:IAO_0000115 "a selectedPlayerAct that involves actions executed by players of the team that currently does not have control of the ball."@en ;
            rdfs:label "outOfPossessionAct"@en .


###  http://www.semanticweb.org/jamesegan/ontologies/2023/9/BasketballOntology/BBO_000016
<http://www.semanticweb.org/jamesegan/ontologies/2023/9/BasketballOntology/BBO_000016> rdf:type owl:Class ;
            rdfs:subClassOf obo:BFO_0000035 ;
            obo:IAO_0000115 "A process boundary that marks the beginning of a basketball game event."@en ;
            rdfs:label "GameStart"@en .

###  http://www.semanticweb.org/jamesegan/ontologies/2023/9/BasketballOntology/BBO_000017
:BBO_000017 rdf:type owl:Class ;
            rdfs:subClassOf obo:BFO_0000035 ;
            obo:IAO_0000115 "A process boundary that marks the end of a basketball game event."@en ;
            rdfs:label "GameEnd"@en .


###  http://www.semanticweb.org/jamesegan/ontologies/2023/9/BasketballOntology/BBO_000018
:BBO_000018 rdf:type owl:Class ;
            rdfs:subClassOf obo:BFO_0000035 ;
            obo:IAO_0000115 "A process boundary that marks the beginning of the first quarter of a basketball game event."@en ;
            rdfs:label "QuarterOneStart"@en .


###  http://www.semanticweb.org/jamesegan/ontologies/2023/9/BasketballOntology/BBO_000019
:BBO_000019 rdf:type owl:Class ;
            rdfs:subClassOf obo:BFO_0000035 ;
            obo:IAO_0000115 "A process boundary that marks the end of the first quarter of a basketball game event."@en ;
            rdfs:label "QuarterOneEnd"@en .


###  http://www.semanticweb.org/jamesegan/ontologies/2023/9/BasketballOntology/BBO_000020
:BBO_000020 rdf:type owl:Class ;
            rdfs:subClassOf obo:BFO_0000035 ;
            obo:IAO_0000115 "A process boundary that marks the beginning of the second quarter of a basketball game event."@en ;
            rdfs:label "QuarterTwoStart"@en .


###  http://www.semanticweb.org/jamesegan/ontologies/2023/9/BasketballOntology/BBO_000021
:BBO_000021 rdf:type owl:Class ;
            rdfs:subClassOf obo:BFO_0000035 ;
            obo:IAO_0000115 "A process boundary that marks the end of the second quarter of a basketball game event."@en ;
            rdfs:label "QuarterTwoEnd"@en .


###  http://www.semanticweb.org/jamesegan/ontologies/2023/9/BasketballOntology/BBO_000022
:BBO_000022 rdf:type owl:Class ;
            rdfs:subClassOf obo:BFO_0000035 ;
            obo:IAO_0000115 "A process boundary that marks the beginning of the third quarter of a basketball game event."@en ;
            rdfs:label "QuarterThreeStart"@en .


###  http://www.semanticweb.org/jamesegan/ontologies/2023/9/BasketballOntology/BBO_000023
:BBO_000023 rdf:type owl:Class ;
            rdfs:subClassOf obo:BFO_0000035 ;
            obo:IAO_0000115 "A process boundary that marks the end of the third quarter of a basketball game event."@en ;
            rdfs:label "QuarterThreeEnd"@en .


###  http://www.semanticweb.org/jamesegan/ontologies/2023/9/BasketballOntology/BBO_000024
:BBO_000024 rdf:type owl:Class ;
            rdfs:subClassOf obo:BFO_0000035 ;
            obo:IAO_0000115 "A process boundary that marks the beginning of the fourth quarter of a basketball game event."@en ;
            rdfs:label "QuarterFourStart"@en .


###  http://www.semanticweb.org/jamesegan/ontologies/2023/9/BasketballOntology/BBO_000025
:BBO_000025 rdf:type owl:Class ;
            rdfs:subClassOf obo:BFO_0000035 ;
            obo:IAO_0000115 "A process boundary that marks the end of the fourth quarter of a basketball game event."@en ;
            rdfs:label "QuarterFourEnd"@en .


###  http://www.semanticweb.org/jamesegan/ontologies/2023/9/BasketballOntology/BBO_000026
:BBO_000026 rdf:type owl:Class ;
            rdfs:subClassOf obo:BFO_0000019 ;
            obo:IAO_0000115 "A quality that a player has measured by units like inches."@en ;
            rdfs:label "Height"@en .


###  http://www.semanticweb.org/jamesegan/ontologies/2023/9/BasketballOntology/BBO_000027
:BBO_000027 rdf:type owl:Class ;
            rdfs:subClassOf obo:BFO_0000019 ;
            obo:IAO_0000115 "A quality that a player has measured by units like pounds."@en ;
            rdfs:label "Weight"@en .
###  Generated by the OWL API (version 4.5.25.2023-02-15T19:15:49Z) https://github.com/owlcs/owlapi
